Remove explicit randomness from SigmaProtocols

code/Decompose.ec
@@ -1,18 +1,11 @@
 (* Formalization of MPC Phi decomposition *)
-require import AllCore Distr SmtMap List.
+require import AllCore Distr List.
 (** Ignore: This is now the preferred setup but is not yet the default **)
 pragma -oldip. pragma +implicits.
-
-type phi = (int -> int).
 
 type input = int.
 type output = int.
 type view = int list.
-
-type input_wires = [
-    UNARY of int
-  | BINARY of (int * int)
-].
 
 type gate = [
   | ADDC of (int * int)
@@ -23,22 +16,18 @@ type gate = [
 
 type circuit = gate list.
 type state = int list.
-(* type input_map = (int, input_wires) fmap. *)
-
-op plus_gate (x y : int) = x + y.
-op mult_gate (x y : int) = x * y.
 
 op eval_gate (g : gate, s : state) : output =
-with g = MULT inputs => let (i, j) = inputs in
-                        let x = (nth 0 s i) in
-                        let y = (nth 0 s j) in x * y
-with g = ADD inputs =>  let (i, j) = inputs in
-                        let x = (nth 0 s i) in
-                        let y = (nth 0 s j) in x + y
-with g = ADDC inputs => let (i, c) = inputs in
-                        let x = (nth 0 s i) in x + c
-with g = MULTC inputs => let (i, c) = inputs in
-                         let x = (nth 0 s i) in x * c.
+  with g = MULT inputs => let (i, j) = inputs in
+                          let x = (nth 0 s i) in
+                          let y = (nth 0 s j) in x * y
+  with g = ADD inputs =>  let (i, j) = inputs in
+                          let x = (nth 0 s i) in
+                          let y = (nth 0 s j) in x + y
+  with g = ADDC inputs => let (i, c) = inputs in
+                          let x = (nth 0 s i) in x + c
+  with g = MULTC inputs => let (i, c) = inputs in
+                          let x = (nth 0 s i) in x * c.
 
 (* Circuit example: *)
 (* x *)
@@ -51,10 +40,6 @@ with g = MULTC inputs => let (i, c) = inputs in
 const circuit_ex = [ADDC (0, 2); MULT(0,1)].
 const s' : state = [10].
 
-(* op eval_circuit(c : circuit, s : state) : output = *)
-(*     with c = [] => last 0 s *)
-(*     with c = g :: gs => let r = eval_gate g s in eval_circuit gs (rcons s r). *)
-
 op eval_circuit_aux(c : circuit, s : state) : state =
     with c = [] => s
     with c = g :: gs =>
@@ -64,17 +49,14 @@ op eval_circuit_aux(c : circuit, s : state) : state =
 op eval_circuit (c : circuit, s : state) : output =
     last 0 (eval_circuit_aux c s).
 
-(* lemma eval_circuit_step g gs s: *)
-(*     eval_circuit (g :: gs) s = eval_circuit gs (rcons s (eval_gate g s)). *)
-(* proof. trivial. qed. *)
-
 lemma circuit_ex_test : (eval_circuit circuit_ex [10]) = 120.
     proof. by rewrite /eval_circuit /circuit_ex /rev /catrev; simplify. qed.
 
 (** Phi protocol **)
 
 (* define decomposed circuit function *)
-type random_tape = int list list.
+type random_tape = int list.
+
 op phi_decomp (g : gate, p : int, w : view list, R : random_tape) : output =
 with g = ADDC inputs =>
     let (i, c) = inputs in
@@ -95,37 +77,26 @@ with g = MULT inputs =>
     let statep = (nth s' w (p - 1)) in
     let xp = (nth 0 statep i) in
     let yp = (nth 0 statep j) in
-    let rp = (nth 0 (nth [] R (p-1)) (size w)) in
+    let rp = (nth 0 R (p-1)) in
     let p = if p = 3 then 0 else p in
     let statep' = (nth s' w (p)) in
     let xp' = (nth 0 statep' i) in
     let yp' = (nth 0 statep' j) in
-    let rp' = (nth 0 (nth [] R p) (size w)) in
+    let rp' = (nth 0 R p) in
     xp * yp + xp' * yp + xp * yp' + rp - rp'.
 
-op phi_circuit_aux (c : circuit, w : view list, R : random_tape) =
-    with c = [] =>
-      let w1 = nth [] w 0 in
-      let w2 = nth [] w 1 in
-      let w3 = nth [] w 2 in (w1, w2, w3)
-    with c = g::gs =>
-      let w1 = nth [] w 0 in
-      let w2 = nth [] w 1 in
-      let w3 = nth [] w 2 in
-      let r1 = phi_decomp g 1 w R in
-      let r2 = phi_decomp g 2 w R in
-      let r3 = phi_decomp g 3 w R in
-      phi_circuit_aux gs [(rcons w1 r1);(rcons w2 r2);(rcons w3 r3)] R.
-
-
-op phi_circuit (c : circuit, w1, w2, w3 : view, R : random_tape) : output =
-    let (w1, w2, w3) = phi_circuit_aux c [w1;w2;w3] R in
-    last 0 w1 + last 0 w2 + last 0 w3.
-
-
-lemma phi_circuit_ex_test R : (phi_circuit circuit_ex [2] [3] [5] R) = 120.
-    proof. rewrite /phi_circuit /circuit_ex /rev.
-    simplify. algebra. qed.
+op simulator_eval (g : gate, p : int, e : int, w : view list, R : random_tape) =
+with g = MULT inputs =>
+  if (e = 1) then (if (p = 2) then (nth 0 R 2) else phi_decomp g 1 w R)
+  else if (e = 2) then (if (p = 2) then (nth 0 R 0) else phi_decomp g 2 ([[]] ++ w) R)
+  else (if (p = 2) then (nth 0 R 1) else phi_decomp g 3 ([(last [] w)]++[[]]++[(head [] w)]) R)
+with g = ADDC inputs =>
+    if (e = 1) then phi_decomp g p w R else
+    if (e = 2) then phi_decomp g (p+1) ([[]] ++ w) R else
+    if (p = 1) then phi_decomp g 3 ([(last [] w)]++[[]]++[(head [] w)]) R else
+    phi_decomp g 1 ([(last [] w)]++[[]]++[(head [] w)]) R
+with g = MULTC inputs => phi_decomp g p w R
+with g = ADD inputs => phi_decomp g p w R.
 
 
 (* secret sharing distribution *)
@@ -135,51 +106,6 @@ lemma dinput_ll : is_lossless dinput by have []:= dinput_llfuni.
 lemma dinput_funi : is_funiform dinput by have []:= dinput_llfuni.
 lemma dinput_fu : is_full dinput by apply/funi_ll_full; [exact/dinput_funi|exact/dinput_ll].
 
-(* Random Oracle *)
-op dtape : {input list distr | is_lossless dtape /\ is_funiform dtape} as dtape_llfuni.
-
-lemma dtape_ll : is_lossless dtape by have []:= dtape_llfuni.
-lemma dtape_funi : is_funiform dtape by have []:= dtape_llfuni.
-lemma dtape_fu : is_full dtape by apply/funi_ll_full; [exact/dtape_funi|exact/dtape_ll].
-
-module Oracle = {
-  proc init(n : int) = {
-    var k, x, tape;
-    tape = [];
-    k = 0;
-    while (k < n) {
-      x <$ dinput;
-      tape = (x::tape);
-      k = k+1;
-    }
-    return tape;
-  }
-
-  proc stepped(n : int) = {
-    var x, tape;
-    tape = init(n-1);
-    if (0 < n) {
-      x <$ dinput;
-      tape = (x::tape);
-    }
-    return tape;
-  }
-}.
-
-equiv init_stepped_equiv:
-    Oracle.init ~ Oracle.stepped : ={n} /\ 0 < n{1} /\ 0 < n{2} ==> ={res}.
-proof.
-  proc. inline *. sp.
-  splitwhile{1} 1 : k < n - 1.
-  unroll{1} 2.
-  seq 1 2 : (={tape, k, n} /\ k{1} = n{1} - 1 /\ 0 < n{1}). auto.
-  while (tape0{2} = tape{1} /\ ={k, n} /\ n0{2} = n{1} - 1 /\ k{1} - 1 < n{1} - 1);
-  auto; progress; smt().
-
-  rcondf{1} 2. auto. if. auto. progress.
-  if. progress. smt().
-  auto. progress.
-qed.
 
 module Phi = {
   proc share(x) = {
@@ -197,13 +123,34 @@ module Phi = {
   proc reconstruct(s1 s2 s3 : int) = {
     return s1 + s2 + s3;
   }
+  proc compute(c : circuit, w1 w2 w3 : view) = {
+    var g, k1, k2, k3, r1, r2, r3;
+    while (c <> []) {
+      g = head (ADDC(0,0)) c;
+      k1 <$ dinput;
+      k2 <$ dinput;
+      k3 <$ dinput;
+      r1 = phi_decomp g 1 [w1;w2;w3] [k1;k2;k3];
+      r2 = phi_decomp g 2 [w1;w2;w3] [k1;k2;k3];
+      r3 = phi_decomp g 3 [w1;w2;w3] [k1;k2;k3];
+      w1 = (rcons w1 r1);
+      w2 = (rcons w2 r2);
+      w3 = (rcons w3 r3);
+      c = behead c;
+    }
+    return (w1, w2, w3);
+  }
+  proc compute_stepped(c : circuit, w1 w2 w3 : view) = {
+    (w1, w2, w3) = compute([head (ADDC(0,0)) c], w1, w2, w3);
+    c = behead c;
+    (w1, w2, w3) = compute(c, w1, w2, w3);
+    return (w1, w2, w3);
+
+  }
   proc main(h : input, c : circuit) = {
-    var x1, x2, x3, y, k1, k2, k3, w1, w2, w3, y1, y2, y3;
+    var x1, x2, x3, y, w1, w2, w3, y1, y2, y3;
     (x1, x2, x3) = share(h);
-    k1 = Oracle.init((size c));
-    k2 = Oracle.init((size c));
-    k3 = Oracle.init((size c));
-    (w1, w2, w3) = phi_circuit_aux c [[x1];[x2];[x3]] [k1;k2;k3];
+    (w1, w2, w3) = compute(c, [x1], [x2], [x3]);
     y1 = output(w1);
     y2 = output(w2);
     y3 = output(w3);
@@ -212,272 +159,468 @@ module Phi = {
   }
 }.
 
-module SampleTest = {
-  proc main() = {
-    var x;
-    x <$ dinput;
-    return x;
+module Simulator = {
+  proc compute(c : circuit, e : int, w1 w2 : view) = {
+    var g, k1, k2, k3, r1, r2;
+    while (c <> []) {
+      g = head (ADDC(0,0)) c;
+      k1 <$ dinput;
+      k2 <$ dinput;
+      k3 <$ dinput;
+      r1 = simulator_eval g 1 e [w1;w2] [k1;k2;k3];
+      r2 = simulator_eval g 2 e [w1;w2] [k1;k2;k3];
+      w1 = (rcons w1 r1);
+      w2 = (rcons w2 r2);
+      c = behead c;
+    }
+
+    return (w1, w2);
+  }
+  proc compute_stepped(c : circuit, e : int, w1 w2 : view) = {
+    (w1, w2) = compute([head (ADDC(0,0)) c], e, w1, w2);
+    c = behead c;
+    (w1, w2) = compute(c, e, w1, w2);
+    return (w1, w2);
+
   }
 }.
 
-lemma oracle_ll_pr:
-    hoare[Oracle.init : true ==> true].
-proof. proc. auto. qed.
+module Privacy = {
+  proc real(h : input, c : circuit, e : int) = {
+    var x1, x2, x3, w1, w2, w3, y1, y2, y3, ret;
+    (x1, x2, x3) = Phi.share(h);
+    (w1, w2, w3) = Phi.compute(c, [x1], [x2], [x3]);
+    y1 = Phi.output(w1);
+    y2 = Phi.output(w2);
+    y3 = Phi.output(w3);
+    if (e = 1) {
+      ret = ((w1, w2), y3);
+    } else {
+      if (e = 2) {
+        ret = ((w2, w3), y1);
+      } else {
+        ret = ((w3, w1), y2);
+      }
+    }
 
-lemma oracle_succedes_pr:
-    (forall (m : int), 0 <= m =>
-    (forall &m, Pr[Oracle.init(m) @ &m : (size res) = m /\ (forall j, j < (size res) /\ 0 <= j => (nth 0 res j) \in dinput) ] = 1%r)).
+    return ret;
+  }
+
+  proc ideal(y : output, c : circuit, e : int) = {
+    var x1, x2, w1, w2, y1, y2, y3;
+    x1 <$ dinput;
+    x2 <$ dinput;
+    (w1, w2) = Simulator.compute(c, e, [x1], [x2]);
+    y1 = Phi.output(w1);
+    y2 = Phi.output(w2);
+    y3 = y - (y1 + y2);
+
+    return ((w1, w2), y3);
+  }
+}.
+
+
+lemma compute_gate_correct g:
+    (forall w1' w2' w3' s s',
+      size s = size w1' /\
+      size s = size w2' /\
+      size s = size w3' /\
+      s' = eval_circuit_aux [g] s =>
+      phoare[Phi.compute : (c = [g] /\ w1 = w1' /\ w2 = w2' /\ w3 = w3' /\
+        (forall i, (nth 0 w1' i) + (nth 0 w2' i) + (nth 0 w3' i) = (nth 0 s i)))
+        ==> let (w1res, w2res, w3res) = res in
+        (forall i, (nth 0 w1res i) + (nth 0 w2res i) + (nth 0 w3res i) = (nth 0 s' i))
+        /\ exists R, w1res = (rcons w1' (phi_decomp g 1 [w1';w2';w3'] R)) /\
+                     w2res = (rcons w2' (phi_decomp g 2 [w1';w2';w3'] R)) /\
+                     w3res = (rcons w3' (phi_decomp g 3 [w1';w2';w3'] R))] = 1%r).
 proof.
-  elim /intind; progress.
-  - byphoare (: n = 0 ==>)=>//. proc. sp. rcondf 1. auto. auto. progress. smt().
-  have -> :
-    Pr[Oracle.init(i+1) @ &m :
-      size res = i+1 /\
-      forall (j : int), j < size res /\ 0 <= j => nth 0 res j \in dinput] =
-    Pr[Oracle.stepped(i+1) @ &m :
-      size res = i+1 /\
-      forall (j : int), j < size res /\ 0 <= j => nth 0 res j \in dinput].
-  byequiv=>//.
-  proc. inline *. sp.
-  splitwhile{1} 1 : k < n - 1.
-  unroll{1} 2.
-  seq 1 2 : (={tape, k, n} /\ k{1} = n{1} - 1 /\ 0 < n{1}). auto.
-  while (tape0{2} = tape{1} /\ ={k, n} /\ n0{2} = n{1} - 1 /\ k{1} - 1 < n{1} - 1);
-  auto; progress; smt().
-  rcondf{1} 2. auto. if. auto. progress.
-  if. progress. smt().
-  auto. progress.
-  have Hph: phoare[Oracle.init : (n = i) ==>
-                size res = i /\
-                forall (j : int), j < size res /\ 0 <= j => nth 0 res j \in dinput] = 1%r.
-  bypr. progress. apply (H0 &m0).
-  byphoare (: n = i + 1 ==>)=>//.
-  proc. case (0 < n).
-  rcondt 2. call oracle_ll_pr. auto.
-  auto.
-  call Hph. auto. progress.
+  progress. proc.
+  rcondt 1. progress.
+  sp. rcondf 11. auto. auto. progress.
   apply dinput_ll.
-  smt().
-  smt().
+  rewrite !nth_rcons.
+  have <- : (size w1{hr} = size w2{hr}) by smt().
+  have <- : (size w1{hr} = size w3{hr}) by smt().
+  rewrite H.
+  case (i < size w1{hr}); progress.
+  apply H2.
+  case (i = size w1{hr}); progress.
+  elim g; progress; smt().
+  by exists [v;v0;v1].
+qed.
 
-  rcondf 2. call oracle_ll_pr. auto.
-  call Hph. auto.
-  smt().
+lemma eval_circuit_aux_size g s:
+    size (eval_circuit_aux [g] s) = size s + 1 by smt.
+
+lemma compute_circuit_correct c':
+    (forall w1' w2' w3' s s',
+      size s = size w1' /\
+      size s = size w2' /\
+      size s = size w3' /\
+      s' = eval_circuit_aux c' s =>
+        phoare[Phi.compute : ( c = c' /\ w1 = w1' /\ w2 = w2' /\ w3 = w3' /\
+                              (forall i, (nth 0 w1' i) + (nth 0 w2' i) + (nth 0 w3' i) = (nth 0 s i)))
+        ==>  let (w1', w2', w3') = res in
+        (forall i, (nth 0 w1' i) + (nth 0 w2' i) + (nth 0 w3' i) = (nth 0 s' i))
+        /\ size s' = size w1' /\ size w1' = size w2' /\ size w2' = size w3'] = 1%r).
+proof.
+  elim c'.
+  - progress. proc. rcondf 1; progress. auto. progress; smt().
+  - move=> x l Hind w1' w2' w3' s s'.
+    move=> [Hs1 [Hs2 [Hs3 Hs'rel]]].
+    bypr=> &m. progress.
+    have -> :
+      Pr[Phi.compute(c{m}, w1{m}, w2{m}, w3{m}) @ &m :
+        let (w1', w2', w3') = res in
+        (forall (i : int),
+            nth 0 w1' i + nth 0 w2' i + nth 0 w3' i =
+          nth 0 s' i)
+        /\ size s' = size w1' /\ size w1' = size w2' /\ size w2' = size w3'] =
+      Pr[Phi.compute_stepped(x::l, w1{m}, w2{m}, w3{m}) @ &m :
+        let (w1', w2', w3') = res in
+        (forall (i : int),
+            nth 0 w1' i + nth 0 w2' i + nth 0 w3' i =
+          nth 0 s' i)
+        /\ size s' = size w1' /\ size w1' = size w2' /\ size w2' = size w3'].
+      + byequiv=>//. clear Hind.
+        proc. inline *. sp.
+        unroll{1} 1; unroll{2} 1.
+        if; progress. smt().
+        + sp. seq 3 3 : (#pre /\ ={k1, k2, k3}); auto.
+          sp. elim *. progress.
+          rcondf{2} 1. progress. sp. elim*. progress.
+          while (c1{2} = c{1} /\ w11{2} = w1{1} /\ w21{2} = w2{1} /\ w31{2} = w3{1}); auto.
+          progress;smt().
+        + exfalso; smt().
+    byphoare(: c = (x::l) /\ w1 = w1{m} /\ w2 = w2{m} /\ w3 = w3{m} ==>)=>//.
+    proc.
+    have Hgate := (compute_gate_correct x w1{m} w2{m} w3{m} s (eval_circuit_aux [x] s) _).
+    do ? split=>//.
+    seq 1 : (
+        (exists R, w1 = rcons w1{m} (phi_decomp x 1 [w1{m}; w2{m}; w3{m}] R) /\
+                   w2 = rcons w2{m} (phi_decomp x 2 [w1{m}; w2{m}; w3{m}] R) /\
+                   w3 = rcons w3{m} (phi_decomp x 3 [w1{m}; w2{m}; w3{m}] R)) /\
+        forall (i : int),
+          nth 0 w1 i + nth 0 w2 i + nth 0 w3 i =
+          nth 0 (eval_circuit_aux [x] s) i /\ c = x :: l).
+    + auto. call Hgate. clear Hgate.
+      skip. move=> *.
+      split; smt().
+
+      elim*; progress.
+      have Hind' := (Hind (rcons w1{m} (phi_decomp x 1 [w1{m}; w2{m}; w3{m}] R))
+                          (rcons w2{m} (phi_decomp x 2 [w1{m}; w2{m}; w3{m}] R))
+                          (rcons w3{m} (phi_decomp x 3 [w1{m}; w2{m}; w3{m}] R)) (eval_circuit_aux [x] s) s' _).
+      do ? split=>//; smt(eval_circuit_aux_size size_rcons).
+      call Hind'. clear Hind Hind'.
+      auto. move=> ? ?.
+      split; smt().
+    + hoare. inline *. sp.
+      rcondt 1. progress.
+      auto. rcondf 12. progress.
+      auto. auto. progress. smt().
+      clear Hgate H Hs'rel. elim x; progress;
+      elim x; move=> x1 x2; rewrite !nth_rcons; smt().
+    trivial.
 qed.
 
 
-lemma oracle_succedes:
-    forall m,
-    0 <= m =>
-    phoare[Oracle.init : (n = m)
-            ==> (size res) = m /\ (forall j, j < (size res) /\ 0 <= j => (nth 0 res j) \in dinput) ] = 1%r.
+lemma phi_sim_equiv g e':
+    (forall w1' w2' w3' s s',
+      size s = size w1' /\
+      size s = size w2' /\
+      size s = size w3' /\
+      s' = eval_circuit_aux [g] s =>
+      equiv[Phi.compute ~ Simulator.compute :
+            (if (e' = 1) then ={w1, w2}
+              else
+              (if (e' = 2) then w2{1} = w1{2} /\ w3{1} = w2{2}
+                else w3{1} = w1{2} /\ w1{1} = w2{2})) /\
+             ={c} /\ e{2} = e' /\ c{1} = [g] /\ w1{1} = w1' /\ w2{1} = w2' /\ w3{1} = w3' /\
+             (forall i, (nth 0 w1' i) + (nth 0 w2' i) + (nth 0 w3' i) = (nth 0 s i))
+            ==>
+            (let (phi_w1, phi_w2, phi_w3) = res{1} in
+              (forall i, (nth 0 phi_w1 i) + (nth 0 phi_w2 i) + (nth 0 phi_w3 i) = (nth 0 s' i)) /\
+              (exists R, phi_w1 = (rcons w1' (phi_decomp g 1 [w1';w2';w3'] R)) /\
+                         phi_w2 = (rcons w2' (phi_decomp g 2 [w1';w2';w3'] R)) /\
+                         phi_w3 = (rcons w3' (phi_decomp g 3 [w1';w2';w3'] R))) /\
+            (if e' = 1 then
+              let (sim_w1, sim_w2) = res{2} in (sim_w1, sim_w2) = (phi_w1, phi_w2)
+            else
+              (if e' = 2 then
+                let (sim_w1, sim_w2) = res{2} in (sim_w1, sim_w2) = (phi_w2, phi_w3)
+              else
+                let (sim_w1, sim_w2) = res{2} in (sim_w1, sim_w2) = (phi_w3, phi_w1))))]).
 proof.
-  progress. bypr.
-  progress. by have := (oracle_succedes_pr n{m} H &m).
+    progress.
+    proc.
+    have Hs1 : size w1' = size w2' by smt().
+    have Hs2 : size w1' = size w3' by smt().
+    rcondt{1} 1. auto.
+    rcondt{2} 1. auto.
+    rcondf{1} 12. auto.
+    rcondf{2} 10. auto.
+    sp. wp.
+    case (e' = 1); progress.
+    seq 2 2 : (#pre /\ ={k1, k2}). auto; smt().
+    elim g; progress; last first.
+    (* Discharge trivial case: ADDC MULTC ADD *)
+    rnd; skip; progress; smt(nth_rcons size_rcons).
+    rnd; skip; progress; smt(nth_rcons size_rcons).
+    rnd; skip; progress; smt(nth_rcons size_rcons).
+    - (* MULT *)
+      elim x=> x1 x2.
+      rnd (fun z => (nth 0 w2{2} x1 * nth 0 w2{2} x2 + nth 0 w3{1} x1 * nth 0 w2{2} x2 + nth 0 w2{2} x1 * nth 0 w3{1} x2 + k2{2} - z)).
+      skip. progress.
+      algebra.
+      apply dinput_funi. smt().
+      algebra.
+      smt(nth_rcons).
+      exists [k1{2};k2{2};k3L].
+      smt().
+      smt().
+      smt().
+    case (e' = 2); progress.
+    (* rnd. rnd. rnd. auto. *)
+    swap 1 2.
+    seq 2 2 : (#pre /\ ={k2, k3}). auto; smt().
+    elim g; progress; last first.
+    (* Discharge trivial case: ADDC MULTC ADD *)
+    rnd; skip; progress; smt(nth_rcons size_rcons).
+    rnd; skip; progress; smt(nth_rcons size_rcons).
+    rnd; skip; progress; smt(nth_rcons size_rcons).
+    - (* MULT *)
+      elim x=> x1 x2.
+      rnd (fun z => (nth 0 w3{1} x1 * nth 0 w3{1} x2 + nth 0 w1{1} x1 * nth 0 w3{1} x2 + nth 0 w3{1} x1 * nth 0 w1{1} x2 + k3{2} - z)).
+      skip. progress.
+      algebra.
+      apply dinput_funi. smt().
+      algebra.
+      smt(nth_rcons).
+      exists [k1L;k2{2};k3{2}].
+      smt().
+      smt().
+      smt().
+    swap 2 1.
+    seq 2 2 : (#pre /\ ={k1, k3}). auto; smt().
+    elim g; progress; last first.
+    (* Discharge trivial case: ADDC MULTC ADD *)
+    rnd; skip; progress; smt(nth_rcons size_rcons).
+    rnd; skip; progress; smt(nth_rcons size_rcons).
+    rnd; skip; progress; smt(nth_rcons size_rcons).
+    - (* MULT *)
+      elim x=> x1 x2.
+      rnd (fun z => (nth 0 w1{1} x1 * nth 0 w1{1} x2 + nth 0 w2{1} x1 * nth 0 w1{1} x2 + nth 0 w1{1} x1 * nth 0 w2{1} x2 + k1{2} - z)).
+      skip. progress.
+      algebra.
+      apply dinput_funi. smt().
+      algebra.
+      smt(nth_rcons).
+      exists [k1{2};k2L;k3{2}].
+      smt().
+      smt().
+      smt().
+      smt().
+      smt().
+      smt().
+      smt().
 qed.
 
-lemma decomp_test &m:
-    Pr[Phi.main(10, circuit_ex) @ &m : res = 120] = 1%r.
+
+lemma phi_sim__circuit_equiv c' e':
+    (forall w1' w2' w3' s s',
+      size s = size w1' /\
+      size s = size w2' /\
+      size s = size w3' /\
+      s' = eval_circuit_aux c' s =>
+      equiv[Phi.compute ~ Simulator.compute :
+            (if (e' = 1) then ={w1, w2}
+              else
+              (if (e' = 2) then w2{1} = w1{2} /\ w3{1} = w2{2}
+                else w3{1} = w1{2} /\ w1{1} = w2{2})) /\
+             ={c} /\ e{2} = e' /\ c{1} = c' /\ w1{1} = w1' /\ w2{1} = w2' /\ w3{1} = w3' /\
+             (forall i, (nth 0 w1' i) + (nth 0 w2' i) + (nth 0 w3' i) = (nth 0 s i))
+            ==>
+            (let (phi_w1, phi_w2, phi_w3) = res{1} in
+              (size phi_w1) = (size phi_w2) /\ (size phi_w2 = size phi_w3) /\
+              (size phi_w1) = (size s') /\
+              (forall i, (nth 0 phi_w1 i) + (nth 0 phi_w2 i) + (nth 0 phi_w3 i) = (nth 0 s' i)) /\
+            (if e' = 1 then
+              let (sim_w1, sim_w2) = res{2} in (sim_w1, sim_w2) = (phi_w1, phi_w2)
+            else
+              (if e' = 2 then
+                let (sim_w1, sim_w2) = res{2} in (sim_w1, sim_w2) = (phi_w2, phi_w3)
+              else
+                let (sim_w1, sim_w2) = res{2} in (sim_w1, sim_w2) = (phi_w3, phi_w1))))]).
 proof.
-    byphoare(: h = 10 /\ c = circuit_ex ==> _)=>//.
-    proc. inline Phi.reconstruct Phi.output Phi.share. auto.
-    have Hsize : 0 <= size circuit_ex by trivial.
-    have H := (oracle_succedes (size circuit_ex) Hsize).
-    call H. call H. call H.
-    auto. progress. apply dinput_ll.
-    rewrite /circuit_ex /phi_circuit /rev. simplify.
-    algebra.
-qed.
-
-lemma decompo_circuit_ex_equiv &m x':
-    Pr[Phi.main(x', circuit_ex) @ &m : res = eval_circuit circuit_ex [x'] ] = 1%r.
-proof.
-    byphoare(: h = x' /\ c = circuit_ex ==> _)=>//.
-    proc. inline Phi.reconstruct Phi.output Phi.share. auto.
-    have Hsize : 0 <= size circuit_ex by trivial.
-    have H := (oracle_succedes (size circuit_ex) Hsize).
-    call H. call H. call H.
-    auto. progress. apply dinput_ll.
-    rewrite /circuit_ex /phi_circuit /rev /eval_circuit. simplify.
-    algebra.
-qed.
-
-lemma circuit_concat gs gs' :
-    (forall s, eval_circuit_aux (gs++gs') s = eval_circuit_aux gs' (eval_circuit_aux gs s)).
-proof. elim gs; progress. by rewrite H. qed.
-
-op tolist (w : (view * view * view)) =
-  let (w1, w2, w3) = w in [w1;w2;w3].
-
-lemma phi_concat gs gs' R:
-    (forall w w1 w2 w3, w = [w1;w2;w3] => phi_circuit_aux (gs++gs') w R = phi_circuit_aux gs' (tolist (phi_circuit_aux gs w R)) R).
-proof. elim gs; rewrite /tolist; progress. smt(). qed.
-
-lemma decomp_equiv g (x x1 x2 x3 : input) (w1 w2 w3 : view) s R:
-    (x = x1 + x2 + x3 /\ (w1,w2,w3) = phi_circuit_aux [g] [[x1];[x2];[x3]] R /\
-    s = eval_circuit_aux [g] [x]) =>
-    (forall i, (nth 0 w1 i) + (nth 0 w2 i) + (nth 0 w3 i) = (nth 0 s i)).
-proof.
-  elim g; progress.
-  - smt().
-  - smt().
-  - elim x0=> x01 x02; case (i = 0); case (i - 1 = 0); case (x01 = 0); case(x02 = 0); progress.
-    algebra. case (x02 = 0). progress. algebra. progress. algebra. case (x01 = 0). progress. algebra.
-    progress. algebra. case (x01 = 0); case (x02 = 0); progress. algebra. algebra.
-    algebra. algebra.
-  - elim x0=> x01 x02; case (i = 0); case (i - 1 = 0); case (x01 = 0); case(x02 = 0); progress.
-    algebra. case (x02 = 0). progress. algebra. progress. case (x01 = 0). progress. algebra.
-    progress. case (x01 = 0); case (x02 = 0); progress. algebra.
-qed.
-
-lemma phi_gate_equiv' g:
-    (forall w1 w2 w3 w1' w2' w3' s' s R,
-      size s = size w1 /\
-      size s = size w2 /\
-      size s = size w3
-      /\ (forall i, (nth 0 w1 i) + (nth 0 w2 i) + (nth 0 w3 i) = (nth 0 s i))
-      /\ (w1',w2',w3') = phi_circuit_aux [g] [w1;w2;w3] R
-      /\ s' = eval_circuit_aux [g] s =>
-      (forall i, (nth 0 w1' i) + (nth 0 w2' i) + (nth 0 w3' i) = (nth 0 s' i))).
-proof.
-   elim g; progress;
-   elim x=> x1 x2;
-   rewrite !nth_rcons;
-   case (i < size w1);
-   case (i < size w2);
-   case (i < size w3);
-   case (i < size s); progress; smt().
-qed.
-
-lemma phi_equiv_ind gs:
-    (forall w1 w2 w3 w1' w2' w3' s' s R,
-      size s = size w1 /\
-      size s = size w2 /\
-      size s = size w3
-      /\ (forall i, (nth 0 w1 i) + (nth 0 w2 i) + (nth 0 w3 i) = (nth 0 s i))
-      /\ (w1',w2',w3') = phi_circuit_aux gs [w1;w2;w3] R
-      /\ s' = eval_circuit_aux gs s =>
-      (forall i, (nth 0 w1' i) + (nth 0 w2' i) + (nth 0 w3' i) = (nth 0 s' i))).
-proof.
-  elim gs. progress. move=> x l H w1 w2 w3 w1' w2' w3' s' s R.
-  move=> [Hs1 [Hs2 [Hs3 [Hrel [Hphi Hcircuit]]]]].
-  have : (w1', w2', w3') = phi_circuit_aux l (tolist (phi_circuit_aux [x] [w1;w2;w3] R)) R by smt().
-  move=> Hphi'.
-  have : s' = eval_circuit_aux l (eval_circuit_aux [x] s) by smt().
-  move=> Hcircuit'.
-  apply (H (rcons w1 (phi_decomp x 1 [w1;w2;w3] R))
-           (rcons w2 (phi_decomp x 2 [w1;w2;w3] R))
-           (rcons w3 (phi_decomp x 3 [w1;w2;w3] R)) (eval_circuit_aux [x] s) R).
-  do split=>//.
-  smt. smt. smt.
-  have :
+  elim c'.
+  - (* empty circuit *)
+    progress.
+    proc.
+    rcondf{1} 1. progress.
+    rcondf{2} 1. progress.
+    skip; progress; smt().
+  - (* Inductive case *)
+    move=> x l IH.
+    move=> w1' w2' w3' s s'.
+    move=> [Hs1 [Hs2 [Hs3 Hs']]].
+    transitivity
+      Phi.compute_stepped
+      (={c, w1, w2, w3} /\
+      c{1} = (x::l) /\ w1{1} = w1' /\ w2{1} = w2' /\ w3{1} = w3'
+      ==> ={res})
+      ((if (e' = 1) then ={w1, w2}
+        else
+        (if (e' = 2) then w2{1} = w1{2} /\ w3{1} = w2{2}
+          else w3{1} = w1{2} /\ w1{1} = w2{2})) /\
+        ={c} /\ e{2} = e' /\ c{1} = (x::l) /\ w1{1} = w1' /\ w2{1} = w2' /\ w3{1} = w3' /\
+        (forall i, (nth 0 w1' i) + (nth 0 w2' i) + (nth 0 w3' i) = (nth 0 s i)) ==>
+          (let (phi_w1, phi_w2, phi_w3) = res{1} in
+            (size phi_w1) = (size phi_w2) /\ (size phi_w2 = size phi_w3) /\
+            (size phi_w1) = (size s') /\
+            (forall i, (nth 0 phi_w1 i) + (nth 0 phi_w2 i) + (nth 0 phi_w3 i) = (nth 0 s' i)) /\
+          (if e' = 1 then
+            let (sim_w1, sim_w2) = res{2} in (sim_w1, sim_w2) = (phi_w1, phi_w2)
+          else
+            (if e' = 2 then
+              let (sim_w1, sim_w2) = res{2} in (sim_w1, sim_w2) = (phi_w2, phi_w3)
+            else
+              let (sim_w1, sim_w2) = res{2} in (sim_w1, sim_w2) = (phi_w3, phi_w1))))).
+    + progress; smt().
+    + progress; smt().
+    + (* proof Phi.compute ~ Phi.compute_stepped *)
+      clear IH. proc. inline *. sp.
+      unroll{1} 1; unroll{2} 1.
+      if; progress.
+      sp. seq 3 3 : (#pre /\ ={k1, k2, k3}); auto.
+      rcondf{2} 8. auto.
+      sp. elim *; progress.
+      while (c1{2} = c{1} /\ w11{2} = w1{1} /\ w21{2} = w2{1} /\ w31{2} = w3{1}); auto.
+      rcondf{1} 1. progress.
+      rcondf{2} 1. progress.
+      rcondf{2} 7. auto.
+      auto.
+  symmetry.
+  transitivity
+    Simulator.compute_stepped
+    (* (={c, e, w1, w2} /\ *)
+    (*   c{1} = (x::l) /\ w1{1} = w1' /\ w2{1} = w2' /\ e{1} = e' *)
+    (={c, w1, w2, e} /\ c{1} = (x::l)
+     ==>
+     ={res})
+    ((if (e' = 1) then ={w1, w2}
+       else
+       (if (e' = 2) then w2{2} = w1{1} /\ w3{2} = w2{1}
+         else w3{2} = w1{1} /\ w1{2} = w2{1})) /\
+       ={c} /\ e{1} = e' /\ c{2} = (x::l) /\ w1{2} = w1' /\ w2{2} = w2' /\ w3{2} = w3' /\
+       (forall i, (nth 0 w1' i) + (nth 0 w2' i) + (nth 0 w3' i) = (nth 0 s i))
+     ==>
+     (let (phi_w1, phi_w2, phi_w3) = res{2} in
+       (size phi_w1) = (size phi_w2) /\ (size phi_w2 = size phi_w3) /\
+       (size phi_w1) = (size s') /\
+       (forall i, (nth 0 phi_w1 i) + (nth 0 phi_w2 i) + (nth 0 phi_w3 i) = (nth 0 s' i)) /\
+     (if e' = 1 then
+       let (sim_w1, sim_w2) = res{1} in (sim_w1, sim_w2) = (phi_w1, phi_w2)
+     else
+       (if e' = 2 then
+         let (sim_w1, sim_w2) = res{1} in (sim_w1, sim_w2) = (phi_w2, phi_w3)
+       else
+         let (sim_w1, sim_w2) = res{1} in (sim_w1, sim_w2) = (phi_w3, phi_w1))))).
+  + progress; smt.
+  + progress; smt.
+  + (* proof Simulator.compute ~ Simulator.compute_stepped *)
+    clear IH. proc. inline *. sp.
+    unroll{1} 1; unroll{2} 1.
+    if; progress.
+    sp. seq 3 3 : (#pre /\ ={k1, k2, k3}); auto.
+    rcondf{2} 6. auto.
+    sp. elim *; progress.
+    while (c1{2} = c{1} /\ e1{2} = e{1} /\ w11{2} = w1{1} /\ w21{2} = w2{1}); auto.
+    rcondf{1} 1. progress.
+    rcondf{2} 1. progress.
+    sp. elim*. progress.
+    rcondf{2} 1. progress.
+    auto.
+  (* main proof *)
+  symmetry.
+  proc.
+  seq 1 1 : (
+      (exists R,  w1{1} = rcons w1' (phi_decomp x 1 [w1'; w2'; w3'] R) /\
+                  w2{1} = rcons w2' (phi_decomp x 2 [w1'; w2'; w3'] R) /\
+                  w3{1} = rcons w3' (phi_decomp x 3 [w1'; w2'; w3'] R)) /\
       (forall (i : int),
-        (nth 0 (rcons w1 (phi_decomp x 1 [w1; w2; w3] R)) i +
-        nth 0 (rcons w2 (phi_decomp x 2 [w1; w2; w3] R)) i +
-        nth 0 (rcons w3 (phi_decomp x 3 [w1; w2; w3] R)) i =
-        nth 0 (eval_circuit_aux [x] s) i) =
-        (if (i < size w1) then
-            nth 0 w1 i +
-            nth 0 w2 i +
-            nth 0 w3 i =
-            nth 0 s i
-         else if (i = size w1) then
-            nth 0 (rcons w1 (phi_decomp x 1 [w1; w2; w3] R)) i +
-            nth 0 (rcons w2 (phi_decomp x 2 [w1; w2; w3] R)) i +
-            nth 0 (rcons w3 (phi_decomp x 3 [w1; w2; w3] R)) i =
-            nth 0 (eval_circuit_aux [x] s) i
-         else 0 = 0)).
-    progress.  clear H.
-    rewrite !nth_rcons. subst.
-    have <- : (size w1 = size w2) by smt().
-    have <- : (size w1 = size w3) by smt().
-    case (i < size w1); progress.
-    case (i = size w1); progress.
-    smt().
-    smt().
-    smt().
-    progress.
-    rewrite H0.
-    case (i < size w1); progress. apply Hrel.
-    have Hgate := (phi_gate_equiv' x).
-    apply (Hgate w1 w2 w3 s R).
-    progress.
-qed.
-
-lemma w_eq_length gs:
-    (forall w1 w2 w3 w1' w2' w3' R,
-      size w1 = size w2 /\ size w2 = size w3 /\
-      (w1',w2',w3') = phi_circuit_aux gs [w1;w2;w3] R =>
-      size w1' = size w2' /\ size w2' = size w3').
-proof.
-  elim gs; progress; smt.
-  (* have Hnew := (H (rcons w1 (phi_decomp x 1 [w1;w2;w3])) *)
-  (*                 (rcons w2 (phi_decomp x 2 [w1;w2;w3])) *)
-  (*                 (rcons w3 (phi_decomp x 3 [w1;w2;w3])) *)
-  (*                 w1' w2' w3'). *)
-qed.
-
-lemma w_s_eq_length gs:
-    (forall w1 w2 w3 w1' w2' w3' s s' R,
-      size w1 = size s /\
-      (w1',w2',w3') = phi_circuit_aux gs [w1;w2;w3] R /\
-      s'  = eval_circuit_aux gs s =>
-      size w1' = size s').
-proof.
-  elim gs; progress; smt.
+        nth 0 w1{1} i + nth 0 w2{1} i + nth 0 w3{1} i =
+        nth 0 (eval_circuit_aux [x] s) i /\ c{1} = x :: l) /\
+      (if (e' = 1) then ={w1, w2}
+        else
+        (if (e' = 2) then w2{1} = w1{2} /\ w3{1} = w2{2}
+          else w3{1} = w1{2} /\ w1{1} = w2{2})) /\
+        ={c} /\ e{2} = e' /\ c{1} = (x::l)).
+   + have Hgate := phi_sim_equiv x e' w1' w2' w3' s (eval_circuit_aux [x] s) _. smt().
+     call Hgate. clear Hgate. clear IH.
+     skip. move=> *.
+     split; smt().
+  elim*. progress.
+  have IH' := (IH (rcons w1' (phi_decomp x 1 [w1'; w2'; w3'] R))
+                  (rcons w2' (phi_decomp x 2 [w1'; w2'; w3'] R))
+                  (rcons w3' (phi_decomp x 3 [w1'; w2'; w3'] R)) (eval_circuit_aux [x] s) s' _).
+  smt(eval_circuit_aux_size size_rcons).
+  call IH'. clear IH IH'.
+  auto. move => *.
+  split; smt().
 qed.
 
 
-(* lemma always_three_views gs: *)
-(*     (forall w1 w2 w3 R, exists w1' w2' w3', *)
-(*       [w1';w2';w3'] = phi_circuit_aux gs [w1;w2;w3] R). *)
-(* proof. *)
-(*   elim gs; progress; [smt | apply H]. *)
-(* qed. *)
-
-
-lemma phi_circuit_equiv &m x' c':
-    Pr[Phi.main(x', c') @ &m : res = eval_circuit c' [x'] ] = 1%r.
+lemma privacy c' x' y' e':
+    y' = eval_circuit c' [x'] =>
+      equiv[Privacy.real ~ Privacy.ideal : (={c, e} /\ c{1} = c' /\ h{1} = x' /\ y{2} = y' /\ e{1} = e')
+            ==> ={res}].
 proof.
-    byphoare(: h = x' /\ c = c' ==> _)=>//.
-    proc. inline Phi.reconstruct Phi.output Phi.share. auto.
-    have Hsize : 0 <= (size c') by smt.
-    have Horacle := (oracle_succedes (size c') Hsize).
-    do ? (call Horacle); auto; progress.
-    apply dinput_ll.
-    rewrite /eval_circuit /phi_circuit /rev.
-    clear Horacle Hsize.
-    have : exists w, w = (phi_circuit_aux c{hr} [[v]; [v0]; [h{hr} - v - v0]] [result;result0;result1]) by smt().
-    elim. move=> w wrel.
-    rewrite - wrel.
-    (* (* have := always_three_views c{hr} [v] [v0] [h{hr} - v - v0] [result;result0;result1]. *) *)
-    (* have : exists w, w = (phi_circuit_aux c{hr} [[v]; [v0]; [h{hr} - v - v0]] [result;result0;result1]) by smt. *)
-    (* progress. *)
-    (* have -> : (nth [] (phi_circuit_aux c{hr} [[v]; [v0]; [h{hr} - v - v0]] [result;result0;result1]) 0) = w1' by smt(). *)
-    (* have -> : (nth [] (phi_circuit_aux c{hr} [[v]; [v0]; [h{hr} - v - v0]] [result;result0;result1]) 1) = w2' by smt(). *)
-    (* have -> : (nth [] (phi_circuit_aux c{hr} [[v]; [v0]; [h{hr} - v - v0]] [result;result0;result1]) 2) = w3' by smt(). *)
-    progress.
-    have :
-      (forall i,
-        (nth 0 w.`1) i +
-        (nth 0 w.`2) i +
-        (nth 0 w.`3) i =
-        (nth 0 (eval_circuit_aux c{hr} [h{hr}]) i)) =>
-      (last 0 w.`1 +
-       last 0 w.`2 +
-       last 0 w.`3 =
-       last 0 (eval_circuit_aux c{hr} [h{hr}])).
-    progress.
-    have Hlast := (last_nth 0 0).
-    rewrite !Hlast.
-    have Heq_len := (w_eq_length c{hr} [v] [v0] [h{hr} - v - v0] w.`1 w.`2 w.`3).
-    have <- : size w.`1 = size w.`2 by smt().
-    have <- : size w.`1 = size w.`3 by smt().
-    have <- : size w.`1 = size (eval_circuit_aux c{hr} [h{hr}]).
-    have Hws_len := w_s_eq_length c{hr} [v] [v0] [h{hr} - v - v0] w.`1 w.`2 w.`3[h{hr}] (eval_circuit_aux c{hr} [h{hr}]) [result;result0;result1].
-    apply Hws_len. smt().
+  progress.
+  proc. inline Phi.output Phi.share.
+  auto.
+
+  case (e' = 1).
+  - seq 5 2 : (#pre /\ ={x1, x2} /\ x' = x1{1} + x2{1} + x3{1}).
+    auto; progress; algebra.
+    exists* x1{1}; exists* x2{1}; exists* x3{1}; elim*; progress.
+    have Heq := phi_sim__circuit_equiv c' e' [x1_L] [x2_L] [x3_L] [x'] (eval_circuit_aux c' [x']) _.
     smt().
-    progress. apply H11. clear H11.
-    have Hrel := (phi_equiv_ind c{hr} [v] [v0] [h{hr} - v - v0] w.`1 w.`2 w.`3 (eval_circuit_aux c{hr} [h{hr}]) [h{hr}] [result;result0;result1]).
-    apply Hrel. smt().
+    call Heq. clear Heq.
+    skip. move=> *.
+    have Hlast := last_nth 0.
+    rewrite /eval_circuit.
+    split; smt().
+
+  case (e' = 2).
+  - seq 5 2 : (#pre /\ x1{2} = x2{1} /\ x3{1} = x2{2} /\ x' = x1{1} + x2{1} + x3{1}).
+    sp; wp.
+    swap{1} 2 - 1.
+    rnd (fun z => h{1} - x20{1} - z).
+    rnd.
+    skip; smt(dinput_funi dinput_fu).
+    exists* x1{1}; exists* x2{1}; exists* x3{1}; elim*; progress.
+    have Heq := phi_sim__circuit_equiv c' e' [x1_L] [x2_L] [x3_L] [x'] (eval_circuit_aux c' [x']) _.
+    smt().
+    call Heq. clear Heq.
+    skip. move=> *.
+    have Hlast := last_nth 0.
+    rewrite /eval_circuit.
+    split; smt().
+
+ (* case e' = 3 *)
+  - seq 5 2 : (#pre /\ x1{2} = x3{1} /\ x1{1} = x2{2} /\ x' = x1{1} + x2{1} + x3{1}).
+    sp; wp.
+    swap{2} 2 - 1.
+    rnd (fun z => h{1} - x10{1} - z).
+    rnd.
+    skip; smt(dinput_funi dinput_fu).
+    exists* x1{1}; exists* x2{1}; exists* x3{1}; elim*; progress.
+    have Heq := phi_sim__circuit_equiv c' e' [x1_L] [x2_L] [x3_L] [x'] (eval_circuit_aux c' [x']) _.
+    smt().
+    call Heq. clear Heq.
+    skip. move=> *.
+    have Hlast := last_nth 0.
+    rewrite /eval_circuit.
+    split; smt().
 qed.
