code/ORProtocol.ec
@@ -13,7 +13,6 @@ theory ORProtocol.
   type witness.
   type message1.
   type message2.
-  type randomness.
   type challenge.
   type response1.
   type response2.
@@ -36,48 +35,45 @@ theory ORProtocol.
   axiom xorA x y : x ^^ y = y ^^ x.
 
   clone SigmaProtocols as S1 with
-    type SigmaProtocols.statement <- statement1,
-    type SigmaProtocols.witness <- witness,
-    type SigmaProtocols.message <- message1,
-    type SigmaProtocols.randomness <- randomness,
-    type SigmaProtocols.challenge <- challenge,
-    type SigmaProtocols.response <- response1,
+    type statement <- statement1,
+    type witness <- witness,
+    type message <- message1,
+    type challenge <- challenge,
+    type response <- response1,
 
-    op SigmaProtocols.R = R1,
-    op SigmaProtocols.dchallenge = dchallenge
+    op R = R1,
+    op dchallenge = dchallenge
     proof *.
-    realize SigmaProtocols.dchallenge_llfuni by apply dchallenge_llfuni.
+    realize dchallenge_llfuni by apply dchallenge_llfuni.
 
   clone SigmaProtocols as S2 with
-    type SigmaProtocols.statement <- statement2,
-    type SigmaProtocols.witness <- witness,
-    type SigmaProtocols.message <- message2,
-    type SigmaProtocols.randomness <- randomness,
-    type SigmaProtocols.challenge <- challenge,
-    type SigmaProtocols.response <- response2,
+    type statement <- statement2,
+    type witness <- witness,
+    type message <- message2,
+    type challenge <- challenge,
+    type response <- response2,
 
-    op SigmaProtocols.R = R2,
-    op SigmaProtocols.dchallenge = dchallenge
+    op R = R2,
+    op dchallenge = dchallenge
     proof *.
-    realize SigmaProtocols.dchallenge_llfuni by apply dchallenge_llfuni.
+    realize dchallenge_llfuni by apply dchallenge_llfuni.
 
   clone SigmaProtocols as Sigma with
-    type SigmaProtocols.statement <- (statement1 * statement2),
-    type SigmaProtocols.witness <- witness,
-    type SigmaProtocols.message <- message,
-    type SigmaProtocols.randomness <- randomness,
-    type SigmaProtocols.challenge <- challenge,
-    type SigmaProtocols.response <- response,
+    type statement <- (statement1 * statement2),
+    type witness <- witness,
+    type message <- message,
+    type challenge <- challenge,
+    type response <- response,
 
-    op SigmaProtocols.R = R,
-    op SigmaProtocols.dchallenge = dchallenge
+    op R = R,
+    op dchallenge = dchallenge
     proof *.
-    realize SigmaProtocols.dchallenge_llfuni by apply dchallenge_llfuni.
+    realize dchallenge_llfuni by apply dchallenge_llfuni.
   export Sigma.
 
 
 
-  module ORProtocol (P1 : S1.SigmaProtocols.SProtocol, P2 : S2.SigmaProtocols.SProtocol) : Sigma.SigmaProtocols.SProtocol = {
+  module ORProtocol (P1 : S1.SProtocol, P2 : S2.SProtocol) : Sigma.SProtocol = {
     var e1 : challenge
     var e2 : challenge
     var z1 : response1
@@ -96,35 +92,35 @@ theory ORProtocol.
       return ret;
     }
 
-    proc init(h : statement, w : witness) : message * randomness = {
-      var h1, h2, r, ret, a1, a2;
+    proc init(h : statement, w : witness) : message = {
+      var h1, h2, ret, a1, a2;
       (h1, h2) = h;
 
       if (R1 h1 w) {
-        (a1, r) = P1.init(h1, w);
+        a1 = P1.init(h1, w);
         e2 <$ dchallenge;
         (a2, z2) = P2.simulator(h2, e2);
-        ret = ((a1, a2), r);
+        ret = (a1, a2);
       } else {
-        (a2, r) = P2.init(h2, w);
+        a2 = P2.init(h2, w);
         e1 <$ dchallenge;
         (a1, z1) = P1.simulator(h1, e1);
-        ret = ((a1, a2), r);
+        ret = (a1, a2);
       }
       return ret;
     }
 
-    proc response(h : statement, w : witness, m : message, r : randomness, s : challenge) : response = {
+    proc response(h : statement, w : witness, m : message, s : challenge) : response = {
       var m1, m2, h1, h2;
       (m1, m2) = m;
       (h1, h2) = h;
 
       if (R1 h1 w) {
         e1 = s ^^ e2;
-        z1 = P1.response(h1, w, m1, r, e1);
+        z1 = P1.response(h1, w, m1, e1);
       } else {
         e2 = s ^^ e1;
-        z2 = P2.response(h2, w, m2, r, e2);
+        z2 = P2.response(h2, w, m2, e2);
       }
       return (e1, z1, e2, z2);
     }
@@ -173,56 +169,56 @@ theory ORProtocol.
 
   }.
 section Security.
-declare module SP1 : S1.SigmaProtocols.SProtocol{ORProtocol}.
-declare module SP2 : S2.SigmaProtocols.SProtocol{ORProtocol,SP1}.
+declare module SP1 : S1.SProtocol{ORProtocol}.
+declare module SP2 : S2.SProtocol{ORProtocol,SP1}.
 
-local module C1 = S1.SigmaProtocols.Completeness(SP1).
-local module C2 = S2.SigmaProtocols.Completeness(SP2).
+local module C1 = S1.Completeness(SP1).
+local module C2 = S2.Completeness(SP2).
 
-local module SHVZK1 = S1.SigmaProtocols.SHVZK(SP1).
-local module SHVZK2 = S2.SigmaProtocols.SHVZK(SP2).
+local module SHVZK1 = S1.SHVZK(SP1).
+local module SHVZK2 = S2.SHVZK(SP2).
 
-  axiom completeness_protocol1 h w e &m : (R1 h w) => Pr[S1.SigmaProtocols.Completeness(SP1).special(h, w, e) @ &m : res] = 1%r.
-  axiom completeness_protocol2 h w e &m : (R2 h w) => Pr[S2.SigmaProtocols.Completeness(SP2).special(h, w, e) @ &m : res] = 1%r.
+  axiom completeness_protocol1 h w e &m : (R1 h w) => Pr[S1.Completeness(SP1).special(h, w, e) @ &m : res] = 1%r.
+  axiom completeness_protocol2 h w e &m : (R2 h w) => Pr[S2.Completeness(SP2).special(h, w, e) @ &m : res] = 1%r.
 
   axiom shvzk1_equiv h' w' e':
-    equiv[S1.SigmaProtocols.SHVZK(SP1).real ~ S1.SigmaProtocols.SHVZK(SP1).ideal : (={h, e} /\ e{1} = e' /\ h{2} = h' /\ w{1} = w' /\ (R1 h' w')) ==> ={res}].
+    equiv[S1.SHVZK(SP1).real ~ S1.SHVZK(SP1).ideal : (={h, e} /\ e{1} = e' /\ h{2} = h' /\ w{1} = w' /\ (R1 h' w')) ==> ={res}].
   axiom shvzk2_equiv h' w' e':
-    equiv[S2.SigmaProtocols.SHVZK(SP2).real ~ S2.SigmaProtocols.SHVZK(SP2).ideal : (={h, e} /\ e{1} = e' /\ h{2} = h' /\ w{1} = w' /\ (R2 h' w')) ==> ={res}].
+    equiv[S2.SHVZK(SP2).real ~ S2.SHVZK(SP2).ideal : (={h, e} /\ e{1} = e' /\ h{2} = h' /\ w{1} = w' /\ (R2 h' w')) ==> ={res}].
 
   local lemma shvzk1_equiv_pr h' w' e' a &m:
       (R1 h' w') =>
-      Pr[S1.SigmaProtocols.SHVZK(SP1).real(h', w', e') @ &m : (res = a)] =
-      Pr[S1.SigmaProtocols.SHVZK(SP1).ideal(h', e') @ &m : (res = a)].
+      Pr[S1.SHVZK(SP1).real(h', w', e') @ &m : (res = a)] =
+      Pr[S1.SHVZK(SP1).ideal(h', e') @ &m : (res = a)].
   proof. move=>rel.
   by byequiv (shvzk1_equiv h' w' e'). qed.
 
   axiom shvzk1_ideal_never_fails_pr h' e' &m:
-      Pr[S1.SigmaProtocols.SHVZK(SP1).ideal(h', e') @ &m : (res <> None)] = 1%r.
+      Pr[S1.SHVZK(SP1).ideal(h', e') @ &m : (res <> None)] = 1%r.
   axiom shvzk2_ideal_never_fails_pr h' e' &m:
-      Pr[S2.SigmaProtocols.SHVZK(SP2).ideal(h', e') @ &m : (res <> None)] = 1%r.
+      Pr[S2.SHVZK(SP2).ideal(h', e') @ &m : (res <> None)] = 1%r.
 
   local lemma shvzk1_ideal_never_fails h' e':
-        phoare[S1.SigmaProtocols.SHVZK(SP1).ideal : (h = h' /\ e = e') ==> (res <> None)] = 1%r.
+        phoare[S1.SHVZK(SP1).ideal : (h = h' /\ e = e') ==> (res <> None)] = 1%r.
   proof. have H := (shvzk1_ideal_never_fails_pr h' e'). bypr. progress. apply (H &m). qed.
 
   local lemma shvzk2_ideal_never_fails h' e':
-        phoare[S2.SigmaProtocols.SHVZK(SP2).ideal : (h = h' /\ e = e') ==> (res <> None)] = 1%r.
+        phoare[S2.SHVZK(SP2).ideal : (h = h' /\ e = e') ==> (res <> None)] = 1%r.
   proof. have H := (shvzk2_ideal_never_fails_pr h' e'). bypr. progress. apply (H &m). qed.
 
   local lemma shvzk1_real_never_fails h' w' e':
-        phoare[S1.SigmaProtocols.SHVZK(SP1).real : (h = h' /\ e = e' /\ w = w' /\ (R1 h' w')) ==> (res <> None)] = 1%r.
+        phoare[S1.SHVZK(SP1).real : (h = h' /\ e = e' /\ w = w' /\ (R1 h' w')) ==> (res <> None)] = 1%r.
   proof.
   bypr. progress.
-  have -> := (S1.SigmaProtocols.shvzk_real_never_fail SP1 h{m} w{m} e{m} &m).
+  have -> := (S1.shvzk_real_never_fail SP1 h{m} w{m} e{m} &m).
   by have := (completeness_protocol1 h{m} w{m} e{m} &m H).
   qed.
 
   local lemma shvzk2_real_never_fails h' w' e':
-        phoare[S2.SigmaProtocols.SHVZK(SP2).real : (h = h' /\ e = e' /\ w = w' /\ (R2 h' w')) ==> (res <> None)] = 1%r.
+        phoare[S2.SHVZK(SP2).real : (h = h' /\ e = e' /\ w = w' /\ (R2 h' w')) ==> (res <> None)] = 1%r.
   proof.
   bypr. progress.
-  have -> := (S2.SigmaProtocols.shvzk_real_never_fail SP2 h{m} w{m} e{m} &m).
+  have -> := (S2.shvzk_real_never_fail SP2 h{m} w{m} e{m} &m).
   by have := (completeness_protocol2 h{m} w{m} e{m} &m H).
   qed.
 
@@ -250,19 +246,19 @@ local module Completeness' = {
   }
 
   proc real1 (h1 : statement1, w : witness, e1 : challenge) : bool = {
-      var a1, r, z1, v1;
+      var a1, z1, v1;
 
-      (a1, r) = SP1.init(h1, w);
-      z1 = SP1.response(h1, w, a1, r, e1);
+      a1 = SP1.init(h1, w);
+      z1 = SP1.response(h1, w, a1, e1);
       v1 = SP1.verify(h1, a1, e1, z1);
       return v1;
   }
 
   proc real2 (h2 : statement2, w : witness, e2) : bool = {
-      var a2, r, z2, v2;
+      var a2, z2, v2;
 
-      (a2, r) = SP2.init(h2, w);
-      z2 = SP2.response(h2, w, a2, r, e2);
+      a2 = SP2.init(h2, w);
+      z2 = SP2.response(h2, w, a2, e2);
       v2 = SP2.verify(h2, a2, e2, z2);
       return v2;
   }
@@ -305,14 +301,14 @@ local module Completeness' = {
   qed.
 
   local lemma completeness_sim_equiv h' w' e' &m:
-      Pr[Sigma.SigmaProtocols.Completeness(ORProtocol(SP1,SP2)).special(h', w', e') @ &m : res] =
+      Pr[Sigma.Completeness(ORProtocol(SP1,SP2)).special(h', w', e') @ &m : res] =
       Pr[Completeness'.main(h', w', e') @ &m : res].
   proof.
     byequiv=>//. proc. inline *. sp. wp.
     case (R1 (fst h') w').
       - rcondt{1} 1. progress.
       - rcondt{2} 1. progress.
-      - rcondt{1} 13. progress. auto. call (: true). rnd. call (: true). auto.
+      - rcondt{1} 12. progress. auto. call (: true). rnd. call (: true). auto.
     swap{2} [5..6] 7.
     swap{2} [5..9] -1.
     swap{1} 1 1.
@@ -322,7 +318,7 @@ local module Completeness' = {
     (* case: R2 is true *)
       - rcondf{1} 1. progress.
       - rcondf{2} 1. progress.
-      - rcondf{1} 13. progress. auto. call (: true). rnd. call (: true). auto.
+      - rcondf{1} 12. progress. auto. call (: true). rnd. call (: true). auto.
     swap{2} [5..6] 6.
     swap{2} [5..9] -1.
     swap{1} 1 1.
@@ -356,13 +352,13 @@ local module Completeness' = {
     move=> rel.
     byphoare (: h = h' /\ e = e' /\ w = w' ==> _)=>//. proc. sp.
     if.
-    - seq 1 : (#pre /\ e2 = e2). auto. auto. progress. apply Sigma.SigmaProtocols.dchallenge_ll.
+    - seq 1 : (#pre /\ e2 = e2). auto. auto. progress. apply Sigma.dchallenge_ll.
       exists* e2. elim*=> e2.
       call (real1_success (fst h') w' (e' ^^ e2)). wp.
       call (ideal2_success (snd h') e2). auto. progress.
       by rewrite xorK.
       hoare. auto. progress.
-    - seq 1 : (#pre /\ e1 = e1). auto. auto. progress. apply Sigma.SigmaProtocols.dchallenge_ll.
+    - seq 1 : (#pre /\ e1 = e1). auto. auto. progress. apply Sigma.dchallenge_ll.
       exists* e1. elim*=> e1.
       call (real2_success (snd h') w' (e' ^^ e1)). wp.
       call (ideal1_success (fst h') e1). auto. progress.
@@ -372,8 +368,8 @@ local module Completeness' = {
   qed.
 
   lemma or_completeness h' w' e' &m:
-      (Sigma.SigmaProtocols.R h' w') =>
-      Pr[Sigma.SigmaProtocols.Completeness(ORProtocol(SP1,SP2)).special(h', w', e') @ &m : res] = 1%r.
+      (Sigma.R h' w') =>
+      Pr[Sigma.Completeness(ORProtocol(SP1,SP2)).special(h', w', e') @ &m : res] = 1%r.
   proof.
     move=> rel.
     have -> := (completeness_sim_equiv h' w' e' &m).
@@ -430,14 +426,14 @@ local module Completeness' = {
     }.
 
   local equiv real_real'_equiv h' w' e':
-    Sigma.SigmaProtocols.SHVZK(ORProtocol(SP1, SP2)).real ~ SHVZK'.real :
+    Sigma.SHVZK(ORProtocol(SP1, SP2)).real ~ SHVZK'.real :
     (h{2} = h' /\ w{2} = w' /\ e{2} = e' /\ (R h' w') /\ ={h, w, e, glob SP1, glob SP2}) ==> ={res}.
   proof.
   proc. inline *. sp. case (R1 (fst h') w').
   (* case: relation is true *)
   rcondt{1} 1. progress.
   rcondt{2} 1. progress.
-  rcondt{1} 13. auto. call (:true). rnd. call(:true). progress.
+  rcondt{1} 12. auto. call (:true). rnd. call(:true). progress.
   sp.
   swap{2} [9..11] 5; swap{1} 2 -1; swap{1} [3..5] 2; swap{2} [9..11] -2.
   do ? (wp; call (: true)).
@@ -446,7 +442,7 @@ local module Completeness' = {
   (* case: relation is false *)
   rcondf{1} 1. progress.
   rcondf{2} 1. progress.
-  rcondf{1} 13. auto. call (:true). rnd. call(:true). progress.
+  rcondf{1} 12. auto. call (:true). rnd. call(:true). progress.
   sp.
   swap{2} [9..11] 5; swap{2} 8 4; swap{2} [8..10] -1; swap{1} 2 -1.
   do ? (wp; call (:true)).
@@ -455,7 +451,7 @@ local module Completeness' = {
   qed.
 
   local equiv ideal_ideal'_equiv h' e':
-    SHVZK'.ideal ~ Sigma.SigmaProtocols.SHVZK(ORProtocol(SP1, SP2)).ideal :
+    SHVZK'.ideal ~ Sigma.SHVZK(ORProtocol(SP1, SP2)).ideal :
     (h{2} = h' /\ e{2} = e' /\ ={h, e, glob SP1, glob SP2}) ==> ={res}.
   proof.
   proc. inline *. sp.
@@ -466,8 +462,8 @@ local module Completeness' = {
   qed.
 
   equiv or_shvzk h' w' e' &m:
-      Sigma.SigmaProtocols.SHVZK(ORProtocol(SP1, SP2)).real ~
-      Sigma.SigmaProtocols.SHVZK(ORProtocol(SP1, SP2)).ideal :
+      Sigma.SHVZK(ORProtocol(SP1, SP2)).real ~
+      Sigma.SHVZK(ORProtocol(SP1, SP2)).ideal :
       (h{2} = h' /\ e{2} = e' /\ ={h, e, glob SP1, glob SP2} /\ w{1} = w' /\ (R h' w')) ==> ={res}.
   proof.
     have ? := (real_real'_equiv h' w' e').
@@ -498,8 +494,8 @@ local module Completeness' = {
     wp. rnd (fun r => r ^^ e{2}) (fun q => q ^^ e{1}).
     auto. progress.
       - by rewrite xorK.
-      - apply Sigma.SigmaProtocols.dchallenge_funi.
-      - apply Sigma.SigmaProtocols.dchallenge_fu.
+      - apply Sigma.dchallenge_funi.
+      - apply Sigma.dchallenge_fu.
       - by rewrite xorK.
       - by rewrite xorA.
       - by rewrite xorA.
@@ -511,13 +507,13 @@ local module Completeness' = {
     ch <> ch' =>
     phoare[SP1.verify : (h = x /\ m = msg /\ e = ch /\ z = d) ==> res] = 1%r =>
     phoare[SP1.verify : (h = x /\ m = msg /\ e = ch' /\ z = d') ==> res] = 1%r =>
-    Pr[S1.SigmaProtocols.SpecialSoundness(SP1).main(x, msg, ch, ch', d, d') @ &m : res] = 1%r.
+    Pr[S1.SpecialSoundness(SP1).main(x, msg, ch, ch', d, d') @ &m : res] = 1%r.
 
   axiom special_soundness_sp2 x msg ch ch' d d' &m :
     ch <> ch' =>
     phoare[SP2.verify : (h = x /\ m = msg /\ e = ch /\ z = d) ==> res] = 1%r =>
     phoare[SP2.verify : (h = x /\ m = msg /\ e = ch' /\ z = d') ==> res] = 1%r =>
-    Pr[S2.SigmaProtocols.SpecialSoundness(SP2).main(x, msg, ch, ch', d, d') @ &m : res] = 1%r.
+    Pr[S2.SpecialSoundness(SP2).main(x, msg, ch, ch', d, d') @ &m : res] = 1%r.
 
   local module SpecialSoundness' = {
       var w : witness
@@ -567,7 +563,7 @@ local module Completeness' = {
   local lemma special_soundness_soundness'_equiv
     x msg ch ch' e1 e1' e2 e2' z1 z1' z2 z2' &m:
       Pr[SpecialSoundness'.main(x, msg, ch, ch', (e1, z1, e2, z2), (e1', z1', e2', z2')) @ &m : res] =
-      Pr[Sigma.SigmaProtocols.SpecialSoundness(ORProtocol(SP1, SP2)).main(x, msg, ch, ch', (e1, z1, e2, z2), (e1', z1', e2', z2')) @ &m : res].
+      Pr[Sigma.SpecialSoundness(ORProtocol(SP1, SP2)).main(x, msg, ch, ch', (e1, z1, e2, z2), (e1', z1', e2', z2')) @ &m : res].
   proof.
     byequiv=>//. proc. inline *. sp.
     case (e1 <> e1').
@@ -647,7 +643,7 @@ local module Completeness' = {
       phoare[SP1.verify : (h = (fst x) /\ m = (fst msg) /\ e = e1' /\ z = z1') ==> res] = 1%r =>
       phoare[SP2.verify : (h = (snd x) /\ m = (snd msg) /\ e = e2 /\ z = z2) ==> res] = 1%r =>
       phoare[SP2.verify : (h = (snd x) /\ m = (snd msg) /\ e = e2' /\ z = z2') ==> res] = 1%r =>
-      Pr[Sigma.SigmaProtocols.SpecialSoundness(ORProtocol(SP1, SP2)).main(x, msg, ch, ch', (e1, z1, e2, z2), (e1', z1', e2', z2')) @ &m : res] = 1%r.
+      Pr[Sigma.SpecialSoundness(ORProtocol(SP1, SP2)).main(x, msg, ch, ch', (e1, z1, e2, z2), (e1', z1', e2', z2')) @ &m : res] = 1%r.
   proof. move=> ch_diff ch_valid ch'_valid accept11 accept12 accept21 accept22.
     have <- := (special_soundness_soundness'_equiv x msg ch ch' e1 e1' e2 e2' z1 z1' z2 z2' &m).
     by have := (special_soundness' x msg ch ch' e1 e1' z1 z1' e2 e2' z2 z2' &m ch_diff ch_valid ch'_valid accept11 accept12 accept21 accept22).
