code/ZKBoo.ec
@@ -1,0 +1,33 @@
+(* Formalization of ZKBoo Sigma-protocol *)
+require import AllCore Distr List DInterval Decompose.
+require (****) SigmaProtocols.
+require import Commitment.
+(** Ignore: This is now the preferred setup but is not yet the default **)
+pragma -oldip. pragma +implicits.
+
+(* TODO index into view *)
+(* TODO constuct random tape *)
+(* pred valid_view w1 w2 k1 k2 = forall j, w1 = phi_decomp *)
+
+type statement  = (circuit * int).
+type witness    = int.
+type message    = output * output * output * commitment * commitment * commitment.
+type challenge  = int.
+type response   = secret_key * secret_key.
+
+op R_DL h w     = let (c, h') = h in (h' = eval_circuit c [w]).
+
+clone import SigmaProtocols as Sigma with
+  type SigmaProtocols.statement <- statement,
+  type SigmaProtocols.witness <- witness,
+  type SigmaProtocols.message <- message,
+  type SigmaProtocols.challenge <- challenge,
+  type SigmaProtocols.response <- response,
+
+  op SigmaProtocols.R = R_DL,
+  op SigmaProtocols.dchallenge = [1..3]
+  proof *.
+  realize SigmaProtocols.dchallenge_llfuni.
+      (* TODO: by [dt_ll, dt_funi] *)
+      split. apply dinter_ll. trivial. apply dinter_uni. qed.
+export SigmaProtocols.
